Correctness via card, ugly proof from GCstep to step (up to renaming)

Launchbury/CardinalityEtaExpandCorrect.thy
@@ -26,7 +26,7 @@ begin
   interpretation supp_bounded_transform transform
     by default (auto simp add: fresh_def supp_transform) 
 
-  type_synonym tstate = "(AEnv \<times> (var \<Rightarrow> two) \<times> Arity \<times> Arity list)"
+  type_synonym tstate = "(AEnv \<times> (var \<Rightarrow> two) \<times> Arity \<times> Arity list \<times> var list)"
 
   fun transform_alts :: "Arity list \<Rightarrow> stack \<Rightarrow> stack"
     where 
@@ -53,22 +53,24 @@ begin
   fun restr_conf :: "var set \<Rightarrow> conf \<Rightarrow> conf"
     where "restr_conf V (\<Gamma>, e, S) = (restrictA V \<Gamma>, e, restr_stack V S)"
 
-  fun conf_transform :: "tstate \<Rightarrow> conf \<Rightarrow> conf"
-  where "conf_transform (ae, ce, a, as) c = a_transform (ae, a, as) (restr_conf (edom ce) c)"
-
+  fun conf_transform :: "tstate \<Rightarrow> conf \<Rightarrow> (var list \<times> conf)"
+  where "conf_transform (ae, ce, a, as, r) c = (r, a_transform (ae, a, as) (restr_conf (- set r) c))"
 
   inductive consistent :: "tstate \<Rightarrow> conf \<Rightarrow> bool" where
     consistentI[intro!]: 
-    "a_consistent (ae, a, as) (restr_conf (edom ce) (\<Gamma>, e, S))
+    "a_consistent (ae, a, as) (restr_conf (- set r) (\<Gamma>, e, S))
     \<Longrightarrow> edom ae = edom ce
     \<Longrightarrow> prognosis ae as a (\<Gamma>, e, S) \<sqsubseteq> ce
     \<Longrightarrow> (\<And> x. x \<in> thunks \<Gamma> \<Longrightarrow> many \<sqsubseteq> ce x \<Longrightarrow> ae x = up\<cdot>0)
-    \<Longrightarrow> consistent (ae, ce, a, as) (\<Gamma>, e, S)"  
+    \<Longrightarrow> set r \<inter> edom ce = {}
+    \<Longrightarrow> set r \<subseteq> domA \<Gamma> \<union> upds S
+    \<Longrightarrow> upds S - edom ce \<subseteq> set r
+    \<Longrightarrow> consistent (ae, ce, a, as, r) (\<Gamma>, e, S)"  
   inductive_cases consistentE[elim!]: "consistent (ae, ce, a, as) (\<Gamma>, e, S)"
 
   lemma closed_consistent:
     assumes "fv e = ({}::var set)"
-    shows "consistent (\<bottom>, \<bottom>, 0, []) ([], e, [])"
+    shows "consistent (\<bottom>, \<bottom>, 0, [], []) ([], e, [])"
   proof-
     from assms
     have "edom (prognosis \<bottom> [] 0 ([], e, [])) = {}"
@@ -78,17 +80,17 @@ begin
   qed
 
   lemma foo:
-    fixes c c' R 
-    assumes "c \<Rightarrow>\<^sup>* c'" and "\<not> boring_step c'" and "consistent (ae,ce,a,as) c"
-    shows "\<exists>ae' ce' a' as'. consistent (ae',ce',a',as') c' \<and> conf_transform (ae,ce,a,as) c \<Rightarrow>\<^sub>G\<^sup>* conf_transform (ae',ce',a',as') c'"
+    fixes c c'
+    assumes "c \<Rightarrow>\<^sup>* c'" and "\<not> boring_step c'" and "consistent (ae,ce,a,as,r) c"
+    shows "\<exists>ae' ce' a' as' r'. consistent (ae',ce',a',as',r') c' \<and> conf_transform (ae,ce,a,as,r) c \<Rightarrow>\<^sub>G\<^sup>* conf_transform (ae',ce',a',as',r') c'"
   using assms
-  proof(induction c c' arbitrary: ae ce a as rule:step_induction)
+  proof(induction c c' arbitrary: ae ce a as r rule:step_induction)
   case (app\<^sub>1 \<Gamma> e x S)
     have "prognosis ae as (inc\<cdot>a) (\<Gamma>, e, Arg x # S) \<sqsubseteq> prognosis ae as a (\<Gamma>, App e x, S)" by (rule prognosis_App)
-    with app\<^sub>1 have "consistent (ae, ce, inc\<cdot>a, as) (\<Gamma>, e, Arg x # S)"
+    with app\<^sub>1 have "consistent (ae, ce, inc\<cdot>a, as, r) (\<Gamma>, e, Arg x # S)"
       by (auto intro: a_consistent_app\<^sub>1 elim: below_trans)
     moreover
-    have "conf_transform (ae, ce, a, as) (\<Gamma>, App e x, S) \<Rightarrow>\<^sub>G conf_transform (ae, ce, inc\<cdot>a, as) (\<Gamma>, e, Arg x # S)"
+    have "conf_transform (ae, ce, a, as, r) (\<Gamma>, App e x, S) \<Rightarrow>\<^sub>G conf_transform (ae, ce, inc\<cdot>a, as, r) (\<Gamma>, e, Arg x # S)"
       by simp rule
     ultimately
     show ?case by (blast del: consistentI consistentE)
@@ -97,10 +99,10 @@ begin
     have "prognosis ae as (pred\<cdot>a) (\<Gamma>, e[y::=x], S) \<sqsubseteq> prognosis ae as a (\<Gamma>, (Lam [y]. e), Arg x # S)"
        by (rule prognosis_subst_Lam)
     then
-    have "consistent (ae, ce, pred\<cdot>a, as) (\<Gamma>, e[y::=x], S)" using app\<^sub>2
+    have "consistent (ae, ce, pred\<cdot>a, as, r) (\<Gamma>, e[y::=x], S)" using app\<^sub>2
       by (auto 4 3 intro: a_consistent_app\<^sub>2 elim: below_trans)
     moreover
-    have "conf_transform (ae, ce, a, as) (\<Gamma>, Lam [y]. e, Arg x # S) \<Rightarrow>\<^sub>G conf_transform (ae, ce, pred \<cdot> a, as) (\<Gamma>, e[y::=x], S)" by (simp add: subst_transform[symmetric]) rule
+    have "conf_transform (ae, ce, a, as, r) (\<Gamma>, Lam [y]. e, Arg x # S) \<Rightarrow>\<^sub>G conf_transform (ae, ce, pred \<cdot> a, as, r) (\<Gamma>, e[y::=x], S)" by (simp add: subst_transform[symmetric]) rule
     ultimately
     show ?case by (blast  del: consistentI consistentE)
   next
@@ -111,6 +113,7 @@ begin
     from thunk have "prognosis ae as a (\<Gamma>, Var x, S) \<sqsubseteq> ce" by auto
     from below_trans[OF prognosis_called fun_belowD[OF this] ]
     have [simp]: "x \<in> edom ce" by (auto simp add: edom_def)
+    hence [simp]: "x \<notin> set r" using thunk by auto
 
     have "x \<notin> upds S" using thunk by (auto dest!: a_consistent_heap_upds_okD  heap_upds_okE)
 
@@ -144,7 +147,7 @@ begin
       have eq: "prognosis (env_delete x ae) as u (delete x \<Gamma>, e, Upd x # S) = prognosis ae as u (delete x \<Gamma>, e, Upd x # S)"
         by (rule prognosis_env_cong) simp
 
-      have [simp]: "restr_stack (edom ce - {x}) S = restr_stack (edom ce) S" 
+      have [simp]: "restr_stack (- set r - {x}) S = restr_stack (- set r) S"
         using `x \<notin> upds S` by (auto intro: restr_stack_cong)
     
       have "prognosis (env_delete x ae) as u (delete x \<Gamma>, e, Upd x # S) \<sqsubseteq> env_delete x ce"
@@ -153,35 +156,36 @@ begin
         by (rule below_env_deleteI)
       moreover
 
-      have *: "a_consistent (env_delete x ae, u, as) (delete x (restrictA (edom ce) \<Gamma>), e, restr_stack (edom ce) S)" using thunk `ae x = up\<cdot>u`
-          by (auto intro!: a_consistent_thunk_once simp del: restr_delete)
+      have *: "a_consistent (env_delete x ae, u, as) (delete x (restrictA (- set r) \<Gamma>), e, restr_stack (- set r) S)"
+        using thunk `ae x = up\<cdot>u`
+        by (auto intro!: a_consistent_thunk_once simp del: restr_delete)
       ultimately
 
-      have "consistent (env_delete x ae, env_delete x ce, u, as) (delete x \<Gamma>, e, Upd x # S)" using thunk
-        by (auto  simp add:   restr_delete_twist elim:below_trans )
+      have "consistent (env_delete x ae, env_delete x ce, u, as, x # r) (delete x \<Gamma>, e, Upd x # S)" using thunk
+        by (auto simp add: restr_delete_twist Compl_insert elim:below_trans )
       moreover
 
       from *
-      have "Astack (transform_alts as (restr_stack (edom ce) S)) \<sqsubseteq> u" by (auto elim: a_consistent_stackD)
+      have "Astack (transform_alts as (restr_stack (- set r) S)) \<sqsubseteq> u" by (auto elim: a_consistent_stackD)
       
       {
       from  `map_of \<Gamma> x = Some e` `ae x = up\<cdot>u` once
-      have "map_of (map_transform Aeta_expand ae (map_transform ccTransform ae (restrictA (edom ce) \<Gamma>))) x = Some (Aeta_expand u (transform u e))"
+      have "map_of (map_transform Aeta_expand ae (map_transform ccTransform ae (restrictA (- set r) \<Gamma>))) x = Some (Aeta_expand u (transform u e))"
         by (simp add: map_of_map_transform)
-      hence "conf_transform (ae, ce, a, as) (\<Gamma>, Var x, S) \<Rightarrow>\<^sub>G
-             (delete x (map_transform Aeta_expand ae (map_transform ccTransform ae (restrictA (edom ce) \<Gamma>))), Aeta_expand u (ccTransform u e), Upd x # transform_alts as (restr_stack (edom ce) S))"
+      hence "conf_transform (ae, ce, a, as, r) (\<Gamma>, Var x, S) \<Rightarrow>\<^sub>G
+             (r, delete x (map_transform Aeta_expand ae (map_transform ccTransform ae (restrictA (- set r) \<Gamma>))), Aeta_expand u (ccTransform u e), Upd x # transform_alts as (restr_stack (- set r) S))"
           by (auto simp add:  map_transform_delete delete_map_transform_env_delete insert_absorb restr_delete_twist simp del: restr_delete)
       also
-      have "\<dots> \<Rightarrow>\<^sub>G\<^sup>* (delete x (map_transform Aeta_expand ae (map_transform ccTransform ae (restrictA (edom ce) \<Gamma>))), Aeta_expand u (ccTransform u e), transform_alts as (restr_stack (edom ce) S))"
+      have "\<dots> \<Rightarrow>\<^sub>G\<^sup>* (x # r, delete x (map_transform Aeta_expand ae (map_transform ccTransform ae (restrictA (- set r) \<Gamma>))), Aeta_expand u (ccTransform u e), transform_alts as (restr_stack (- set r) S))"
         by (rule r_into_rtranclp, rule)
       also
-      have "\<dots> \<Rightarrow>\<^sub>G\<^sup>* (delete x (map_transform Aeta_expand ae (map_transform ccTransform ae  (restrictA (edom ce) \<Gamma>))), ccTransform u e, transform_alts as (restr_stack (edom ce) S))"
-        by (intro normal_trans Aeta_expand_correct `Astack (transform_alts as (restr_stack (edom ce) S)) \<sqsubseteq> u`)
+      have "\<dots> \<Rightarrow>\<^sub>G\<^sup>* (x # r, delete x (map_transform Aeta_expand ae (map_transform ccTransform ae  (restrictA (- set r) \<Gamma>))), ccTransform u e, transform_alts as (restr_stack (- set r) S))"
+        by (intro normal_trans Aeta_expand_correct `Astack (transform_alts as (restr_stack (- set r) S)) \<sqsubseteq> u`)
       also(rtranclp_trans)
-      have "\<dots> = conf_transform (env_delete x ae, env_delete x ce, u, as) (delete x \<Gamma>, e, Upd x # S)" 
-        by (auto intro!: map_transform_cong simp add:  map_transform_delete[symmetric]  restr_delete_twist)
+      have "\<dots> = conf_transform (env_delete x ae, env_delete x ce, u, as, x # r) (delete x \<Gamma>, e, Upd x # S)" 
+        by (auto intro!: map_transform_cong simp add:  map_transform_delete[symmetric]  restr_delete_twist Compl_insert)
       finally(back_subst)
-      have "conf_transform (ae, ce, a, as) (\<Gamma>, Var x, S) \<Rightarrow>\<^sub>G\<^sup>* conf_transform (env_delete x ae, env_delete x ce, u, as) (delete x \<Gamma>, e, Upd x # S)".
+      have "conf_transform (ae, ce, a, as, r) (\<Gamma>, Var x, S) \<Rightarrow>\<^sub>G\<^sup>* conf_transform (env_delete x ae, env_delete x ce, u, as, x # r) (delete x \<Gamma>, e, Upd x # S)".
       }
       ultimately
       show ?thesis by (blast del: consistentI consistentE)
@@ -202,18 +206,18 @@ begin
       
       have "prognosis ae as 0 (delete x \<Gamma>, e, Upd x # S) \<sqsubseteq> ce" using *[unfolded `u=0`] thunk by (auto elim: below_trans)
       moreover
-      have "a_consistent (ae, 0, as) (delete x (restrictA (edom ce) \<Gamma>), e, Upd x # restr_stack (edom ce) S)" using thunk `ae x = up\<cdot>0`
+      have "a_consistent (ae, 0, as) (delete x (restrictA (- set r) \<Gamma>), e, Upd x # restr_stack (- set r) S)" using thunk `ae x = up\<cdot>0`
         by (auto intro!: a_consistent_thunk_0 simp del: restr_delete)
       ultimately
-      have "consistent (ae, ce, 0, as) (delete x \<Gamma>, e, Upd x # S)" using thunk `ae x = up\<cdot>u` `u = 0`
+      have "consistent (ae, ce, 0, as, r) (delete x \<Gamma>, e, Upd x # S)" using thunk `ae x = up\<cdot>u` `u = 0`
         by (auto simp add:  restr_delete_twist)
       moreover
   
       from  `map_of \<Gamma> x = Some e` `ae x = up\<cdot>0` many
-      have "map_of (map_transform Aeta_expand ae (map_transform ccTransform ae (restrictA (edom ce) \<Gamma>))) x = Some (transform 0 e)"
+      have "map_of (map_transform Aeta_expand ae (map_transform ccTransform ae (restrictA (- set r) \<Gamma>))) x = Some (transform 0 e)"
         by (simp add: map_of_map_transform)
       with `\<not> isVal e`
-      have "conf_transform (ae, ce, a, as) (\<Gamma>, Var x, S) \<Rightarrow>\<^sub>G conf_transform (ae, ce, 0, as) (delete x \<Gamma>, e, Upd x # S)"
+      have "conf_transform (ae, ce, a, as, r) (\<Gamma>, Var x, S) \<Rightarrow>\<^sub>G conf_transform (ae, ce, 0, as, r) (delete x \<Gamma>, e, Upd x # S)"
         by (auto simp add: map_transform_delete restr_delete_twist intro!: step.intros  simp del: restr_delete)
       ultimately
       show ?thesis by (blast del: consistentI consistentE)
@@ -227,6 +231,9 @@ begin
     have [simp]: "x \<in> edom ce" by (auto simp add: edom_def)
     then obtain c where "ce x = up\<cdot>c" by (cases "ce x") (auto simp add: edom_def)
 
+    from lamvar
+    have [simp]: "x \<notin> set r" by auto
+
     then have "x \<in> edom ae" using lamvar by auto
     then obtain  u where "ae x = up\<cdot>u"  by (cases "ae x") (auto simp add: edom_def)
 
@@ -238,15 +245,15 @@ begin
     also have "\<dots> \<sqsubseteq> prognosis ae as a (\<Gamma>, Var x, S)" by (rule record_call_below_arg)
     finally have *: "prognosis ae as u ((x, e) # delete x \<Gamma>, e, S) \<sqsubseteq> prognosis ae as a (\<Gamma>, Var x, S)" by this simp_all
     moreover
-    have "a_consistent (ae, u, as) ((x,e) # delete x (restrictA (edom ce) \<Gamma>), e, restr_stack (edom ce) S)" using lamvar `ae x = up\<cdot>u`
+    have "a_consistent (ae, u, as) ((x,e) # delete x (restrictA (- set r) \<Gamma>), e, restr_stack (- set r) S)" using lamvar `ae x = up\<cdot>u`
       by (auto intro!: a_consistent_lamvar simp del: restr_delete)
     ultimately
-    have "consistent (ae, ce, u, as) ((x, e) # delete x \<Gamma>, e, S)"
+    have "consistent (ae, ce, u, as, r) ((x, e) # delete x \<Gamma>, e, S)"
       using lamvar edom_mono[OF *] by (auto simp add:  thunks_Cons restr_delete_twist elim: below_trans)
     moreover
 
     from `a_consistent _ _`
-    have "Astack (transform_alts as (restr_stack (edom ce) S)) \<sqsubseteq> u" by (auto elim: a_consistent_stackD)
+    have "Astack (transform_alts as (restr_stack (- set r) S)) \<sqsubseteq> u" by (auto elim: a_consistent_stackD)
   
     {
     from `isVal e`
@@ -254,19 +261,19 @@ begin
     hence "isVal (Aeta_expand u (transform u e))" by (rule isVal_Aeta_expand)
     moreover
     from  `map_of \<Gamma> x = Some e`  `ae x = up \<cdot> u` `ce x = up\<cdot>c` `isVal (transform u e)`
-    have "map_of (map_transform Aeta_expand ae (map_transform transform ae (restrictA (edom ce) \<Gamma>))) x = Some (Aeta_expand u (transform u e))"
+    have "map_of (map_transform Aeta_expand ae (map_transform transform ae (restrictA (- set r) \<Gamma>))) x = Some (Aeta_expand u (transform u e))"
       by (simp add: map_of_map_transform)
     ultimately
-    have "conf_transform (ae, ce, a, as) (\<Gamma>, Var x, S) \<Rightarrow>\<^sup>*
-          ((x, Aeta_expand u (transform u e)) # delete x (map_transform Aeta_expand ae (map_transform transform ae (restrictA (edom ce) \<Gamma>))), Aeta_expand u (transform u e), transform_alts as (restr_stack (edom ce) S))"
-       by (auto intro: lambda_var simp add: map_transform_delete simp del: restr_delete)
-    also have "\<dots> = ((map_transform Aeta_expand ae (map_transform transform ae ((x,e) # delete x (restrictA (edom ce) \<Gamma>)))), Aeta_expand u  (transform u e), transform_alts as (restr_stack (edom ce) S))"
+    have "conf_transform (ae, ce, a, as, r) (\<Gamma>, Var x, S) \<Rightarrow>\<^sub>G\<^sup>*
+          (r, (x, Aeta_expand u (transform u e)) # delete x (map_transform Aeta_expand ae (map_transform transform ae (restrictA (- set r) \<Gamma>))), Aeta_expand u (transform u e), transform_alts as (restr_stack (- set r) S))"
+       by (auto intro!: normal_trans[OF lambda_var] simp add: map_transform_delete simp del: restr_delete)
+    also have "\<dots> = (r, (map_transform Aeta_expand ae (map_transform transform ae ((x,e) # delete x (restrictA (- set r) \<Gamma>)))), Aeta_expand u  (transform u e), transform_alts as (restr_stack (- set r) S))"
       using `ae x = up \<cdot> u` `ce x = up\<cdot>c` `isVal (transform u e)`
       by (simp add: map_transform_Cons map_transform_delete restr_delete_twist del: restr_delete)
-    also(subst[rotated]) have "\<dots> \<Rightarrow>\<^sup>* conf_transform (ae, ce, u, as) ((x, e) # delete x \<Gamma>, e, S)"
-      by (simp add: restr_delete_twist) (rule Aeta_expand_correct[OF `Astack _ \<sqsubseteq> u`])
+    also(subst[rotated]) have "\<dots> \<Rightarrow>\<^sub>G\<^sup>* conf_transform (ae, ce, u, as, r) ((x, e) # delete x \<Gamma>, e, S)"
+      by (simp add: restr_delete_twist) (rule normal_trans[OF Aeta_expand_correct[OF `Astack _ \<sqsubseteq> u`]])
     finally(rtranclp_trans)
-    have "conf_transform (ae, ce, a, as) (\<Gamma>, Var x, S) \<Rightarrow>\<^sup>* conf_transform (ae, ce, u, as) ((x, e) # delete x \<Gamma>, e, S)".
+    have "conf_transform (ae, ce, a, as, r) (\<Gamma>, Var x, S) \<Rightarrow>\<^sub>G\<^sup>* conf_transform (ae, ce, u, as, r) ((x, e) # delete x \<Gamma>, e, S)".
     }
     ultimately show ?case by (blast intro: normal_trans del: consistentI consistentE)
   next
@@ -274,28 +281,25 @@ begin
     show ?case
     proof(cases "x \<in> edom ce")
       case True[simp]
-      hence "ce x \<noteq> \<bottom>" using var\<^sub>2 by (auto simp add: edom_def)
-      from True have "x \<in> edom ae" using var\<^sub>2 by auto
- 
-      obtain c where "ce x = up\<cdot>c" using `ce x \<noteq> \<bottom>` by (cases "ce x") auto
-  
+      hence [simp]: "x \<notin> set r" using var\<^sub>2 by auto
+
       from var\<^sub>2
-      have "a_consistent (ae, a, as) (restrictA (edom ce) \<Gamma>, e, Upd x # restr_stack (edom ce) S)" by auto
-      from a_consistent_UpdD[OF this  `x \<in> edom ae`]
+      have "a_consistent (ae, a, as) (restrictA (- set r) \<Gamma>, e, Upd x # restr_stack (-set r) S)" by auto
+      from a_consistent_UpdD[OF this]
       have "ae x = up\<cdot>0" and "a = 0".
   
       from `isVal e` `x \<notin> domA \<Gamma>`
       have *: "prognosis ae as 0 ((x, e) # \<Gamma>, e, S) \<sqsubseteq> prognosis ae as 0 (\<Gamma>, e, Upd x # S)" by (rule prognosis_Var2)
       moreover
-      have "a_consistent (ae, a, as) ((x, e) # restrictA (edom ce) \<Gamma>, e, restr_stack (edom ce) S)"
+      have "a_consistent (ae, a, as) ((x, e) # restrictA (- set r) \<Gamma>, e, restr_stack (- set r) S)"
         using var\<^sub>2 by (auto intro!: a_consistent_var\<^sub>2)
       ultimately
-      have "consistent (ae, ce, 0, as) ((x, e) # \<Gamma>, e, S)"
+      have "consistent (ae, ce, 0, as, r) ((x, e) # \<Gamma>, e, S)"
         using var\<^sub>2 `a = 0`
         by (auto simp add: thunks_Cons elim: below_trans)
       moreover
-      have "conf_transform (ae, ce, a, as) (\<Gamma>, e, Upd x # S) \<Rightarrow>\<^sub>G conf_transform (ae, ce, 0, as) ((x, e) # \<Gamma>, e, S)"
-        using `ae x = up\<cdot>0` `a = 0` var\<^sub>2 `ce x = up\<cdot>c`
+      have "conf_transform (ae, ce, a, as, r) (\<Gamma>, e, Upd x # S) \<Rightarrow>\<^sub>G conf_transform (ae, ce, 0, as, r) ((x, e) # \<Gamma>, e, S)"
+        using `ae x = up\<cdot>0` `a = 0` var\<^sub>2 
         by (auto intro!: step.intros simp add: map_transform_Cons)
       ultimately show ?thesis by (blast del: consistentI consistentE)
     next
@@ -305,23 +309,22 @@ begin
       from False have "x \<notin> edom ae" using var\<^sub>2 by auto
       hence [simp]: "ae x = \<bottom>" by (auto simp add: edom_def)
 
+      from False have [simp]: "x \<in> set r" using var\<^sub>2 by auto
       
       have "prognosis ae as a ((x, e) # \<Gamma>, e, S) \<sqsubseteq> prognosis ae as a ((x, e) # \<Gamma>, e, Upd x # S)" by (rule prognosis_upd)
-      also
-       
-      from `ae x = \<bottom>`
-      have "prognosis ae as a ((x, e) # \<Gamma>, e, Upd x # S) \<sqsubseteq> prognosis ae as a (delete x ((x,e) # \<Gamma>), e, Upd x # S)"
-        by (rule prognosis_not_called)
-      also have  "delete x ((x,e)#\<Gamma>) = \<Gamma>" using `x \<notin> domA \<Gamma>` by simp
+      also have "\<dots> \<sqsubseteq> prognosis ae as a (delete x ((x,e) # \<Gamma>), e, Upd x # S)"
+        using `ae x = \<bottom>` by (rule prognosis_not_called)
+      also have "delete x ((x,e)#\<Gamma>) = \<Gamma>" using `x \<notin> domA \<Gamma>` by simp
       finally
       have *: "prognosis ae as a ((x, e) # \<Gamma>, e, S) \<sqsubseteq> prognosis ae as a (\<Gamma>, e, Upd x # S)" by this simp
       then
-      have "consistent (ae, ce, a, as) ((x, e) # \<Gamma>, e, S)" using var\<^sub>2
-        by (auto simp add: thunks_Cons  elim:below_trans)
+      have "consistent (ae, ce, a, as, r) ((x, e) # \<Gamma>, e, S)" using var\<^sub>2
+        by (auto simp add: thunks_Cons  elim:below_trans a_consistent_var\<^sub>2)
       moreover
-      have "conf_transform (ae, ce, a, as) (\<Gamma>, e, Upd x # S) = conf_transform (ae, ce, a, as) ((x, e) # \<Gamma>, e, S)"
-        by(simp add: map_transform_restrA[symmetric])
-      ultimately show ?thesis by (auto del: consistentI consistentE simp del:conf_transform.simps)
+      have "conf_transform (ae, ce, a, as, r) (\<Gamma>, e, Upd x # S) = conf_transform (ae, ce, a, as, r) ((x, e) # \<Gamma>, e, S)"
+        by (auto simp add: map_transform_restrA[symmetric])
+      ultimately show ?thesis
+        by (fastforce del: consistentI consistentE simp del:conf_transform.simps)
     qed
   next
     case (let\<^sub>1 \<Delta> \<Gamma> e S)
@@ -345,6 +348,12 @@ begin
     from fresh_distinct[OF let\<^sub>1(1)]
     have [simp]: "restrictA (edom ae \<union> edom (Aheap \<Delta> e\<cdot>a)) \<Gamma> = restrictA (edom ae) \<Gamma>"
       by (auto intro: restrictA_cong dest!: set_mp[OF edom_Aheap]) 
+
+    have "set r \<subseteq> domA \<Gamma> \<union> upds S" using let\<^sub>1 by auto
+    have [simp]: "restrictA (- set r) \<Delta> = \<Delta>"
+      apply (rule restrictA_noop)
+      apply auto
+      by (metis IntI UnE `set r \<subseteq> domA \<Gamma> \<union> upds S` `domA \<Delta> \<inter> domA \<Gamma> = {}` `domA \<Delta> \<inter> upds S = {}` contra_subsetD empty_iff)
 
     {
     have "edom (?ae \<squnion> ae) = edom (?ce \<squnion> ce)"
@@ -380,27 +389,29 @@ begin
     finally have "prognosis (?ae \<squnion> ae) as a (\<Delta> @ \<Gamma>, e, S) \<sqsubseteq> ?ce \<squnion> ce" by this simp
     }
     moreover
-    
-    have "a_consistent (ae, a, as) (restrictA (edom ce) \<Gamma>, Let \<Delta> e, restr_stack (edom ce) S)"
+
+    have "a_consistent (ae, a, as) (restrictA (- set r) \<Gamma>, Let \<Delta> e, restr_stack (- set r) S)"
       using let\<^sub>1 by auto
-    hence "a_consistent (?ae \<squnion> ae, a, as) (\<Delta> @ restrictA (edom ce) \<Gamma>, e, restr_stack (edom ce) S)"
+    hence "a_consistent (?ae \<squnion> ae, a, as) (\<Delta> @ restrictA (- set r) \<Gamma>, e, restr_stack (- set r) S)"
       using let\<^sub>1(1,2) `edom ae \<inter> domA \<Delta> = {}` 
       by (auto intro!:  a_consistent_let simp del: join_comm)
-    hence "a_consistent (?ae \<squnion> ae, a, as) (restrictA (edom (?ae \<squnion> ae)) (\<Delta> @ restrictA (edom ce) \<Gamma>), e, restr_stack (edom ce) S)"
-      by (rule a_consistent_restrictA[OF _ order_refl])
-    hence "a_consistent (?ae \<squnion> ae, a, as) (restrictA (edom (?ce \<squnion> ce)) (\<Delta> @ \<Gamma>), e, restr_stack (edom (?ce \<squnion> ce)) S)"
-      by (simp add: restrictA_append restr_stack_simp2[simplified] edom_cHeap `edom ce = edom ae` Int_Un_distrib2)
+    hence "a_consistent (?ae \<squnion> ae, a, as) (restrictA (- set r) (\<Delta> @ \<Gamma>), e, restr_stack (- set r) S)"
+      by (simp add: restrictA_append)
+    moreover
+    have "set r \<inter> edom ce = {}" and "upds S - edom ce \<subseteq> set r" and "set r \<subseteq> domA \<Gamma> \<union> upds S" using let\<^sub>1 by auto
+    hence "set r \<inter> edom (?ce \<squnion> ce) = {}" and "upds S - edom (?ce \<squnion> ce) \<subseteq> set r"  and "set r \<subseteq> domA \<Gamma> \<union> upds S"
+      apply (auto simp add: edom_cHeap dest!: set_mp[OF edom_Aheap])
+      by (metis IntI UnE `domA \<Delta> \<inter> domA \<Gamma> = {}` `domA \<Delta> \<inter> upds S = {}` contra_subsetD empty_iff)
     ultimately
-    have "consistent (?ae \<squnion> ae, ?ce \<squnion> ce, a, as) (\<Delta> @ \<Gamma>, e, S)"
-      by auto
+    have "consistent (?ae \<squnion> ae, ?ce \<squnion> ce, a, as, r) (\<Delta> @ \<Gamma>, e, S)" by auto
     }
     moreover
     {
       have "\<And> x. x \<in> domA \<Gamma> \<Longrightarrow> x \<notin> edom ?ae" "\<And> x. x \<in> domA \<Gamma> \<Longrightarrow> x \<notin> edom ?ce"
         using fresh_distinct[OF let\<^sub>1(1)]
         by (auto simp add: edom_cHeap dest!: set_mp[OF edom_Aheap])
-      hence "map_transform Aeta_expand (?ae \<squnion> ae) (map_transform transform (?ae \<squnion> ae) (restrictA (edom (?ce \<squnion> ce)) \<Gamma>))
-         = map_transform Aeta_expand ae (map_transform transform ae (restrictA (edom ce) \<Gamma>))"
+      hence "map_transform Aeta_expand (?ae \<squnion> ae) (map_transform transform (?ae \<squnion> ae) (restrictA (-set r) \<Gamma>))
+         = map_transform Aeta_expand ae (map_transform transform ae (restrictA (-set r) \<Gamma>))"
          by (auto intro!: map_transform_cong restrictA_cong simp add: edomIff)
       moreover
   
@@ -408,16 +419,16 @@ begin
       have "\<And> x. x \<in> domA \<Delta> \<Longrightarrow> x \<notin> edom ce" and  "\<And> x. x \<in> domA \<Delta> \<Longrightarrow> x \<notin> edom ae"
          using fresh_distinct[OF let\<^sub>1(1)] fresh_distinct_fv[OF let\<^sub>1(2)] 
          by (auto dest!:  set_mp[OF ups_fv_subset])
-      hence "map_transform Aeta_expand (?ae \<squnion> ae) (map_transform transform (?ae \<squnion> ae) (restrictA (edom (?ce \<squnion> ce)) \<Delta>))
-         = map_transform Aeta_expand ?ae (map_transform transform ?ae (restrictA (edom ?ce) \<Delta>))"
+      hence "map_transform Aeta_expand (?ae \<squnion> ae) (map_transform transform (?ae \<squnion> ae) (restrictA (- set r) \<Delta>))
+         = map_transform Aeta_expand ?ae (map_transform transform ?ae (restrictA (- set r) \<Delta>))"
          by (auto intro!: map_transform_cong restrictA_cong simp add: edomIff)
       ultimately
       
       
-      have "conf_transform (ae, ce, a, as) (\<Gamma>, Let \<Delta> e, S) \<Rightarrow>\<^sub>G\<^sup>* conf_transform (?ae \<squnion> ae, ?ce \<squnion> ce, a, as) (\<Delta> @ \<Gamma>, e, S)"
+      have "conf_transform (ae, ce, a, as, r) (\<Gamma>, Let \<Delta> e, S) \<Rightarrow>\<^sub>G conf_transform (?ae \<squnion> ae, ?ce \<squnion> ce, a, as, r) (\<Delta> @ \<Gamma>, e, S)"
         using restr_stack_simp2 let\<^sub>1(1,2) `edom ce = edom ae`
-        apply (auto simp add: map_transform_append restrictA_append edom_cHeap restr_stack_simp2[simplified] map_transform_restrA)
-        apply (rule let_and_restrict)
+        apply (auto simp add: map_transform_append restrictA_append edom_cHeap restr_stack_simp2[simplified] )
+        apply (rule normal[OF  step.let\<^sub>1])
         apply (auto dest: set_mp[OF edom_Aheap])
         done
     }
@@ -428,16 +439,16 @@ begin
     have "prognosis ae as a (\<Gamma>, scrut ? e1 : e2, S) \<sqsubseteq> ce" using if\<^sub>1 by auto
     hence "prognosis ae (a#as) 0 (\<Gamma>, scrut, Alts e1 e2 # S) \<sqsubseteq> ce"
       by (rule below_trans[OF prognosis_IfThenElse])
-    hence "consistent (ae, ce, 0, a#as) (\<Gamma>, scrut, Alts e1 e2 # S)"
+    hence "consistent (ae, ce, 0, a#as, r) (\<Gamma>, scrut, Alts e1 e2 # S)"
       using if\<^sub>1  by (auto dest: a_consistent_if\<^sub>1)
     moreover
-    have "conf_transform (ae, ce, a, as) (\<Gamma>, scrut ? e1 : e2, S) \<Rightarrow>\<^sub>G conf_transform (ae, ce, 0, a#as) (\<Gamma>, scrut, Alts e1 e2 # S)"
+    have "conf_transform (ae, ce, a, as, r) (\<Gamma>, scrut ? e1 : e2, S) \<Rightarrow>\<^sub>G conf_transform (ae, ce, 0, a#as, r) (\<Gamma>, scrut, Alts e1 e2 # S)"
       by (auto intro: normal step.intros)
     ultimately
     show ?case by (blast del: consistentI consistentE)
   next
     case (if\<^sub>2 \<Gamma> b e1 e2 S)
-    hence "a_consistent (ae, a, as) (restrictA (edom ce) \<Gamma>, Bool b, Alts e1 e2 # restr_stack (edom ce) S)" by auto
+    hence "a_consistent (ae, a, as) (restrictA (- set r) \<Gamma>, Bool b, Alts e1 e2 # restr_stack (-set r) S)" by auto
     then  obtain a' as' where [simp]: "as = a' # as'" "a = 0"
       by (rule a_consistent_alts_on_stack)
 
@@ -445,22 +456,24 @@ begin
     have "prognosis ae (a'#as') 0 (\<Gamma>, Bool b, Alts e1 e2 # S) \<sqsubseteq> ce" using if\<^sub>2 by auto
     hence "prognosis ae as' a' (\<Gamma>, if b then e1 else e2, S) \<sqsubseteq> ce" by (rule below_trans[OF prognosis_Alts])
     then
-    have "consistent (ae, ce, a', as') (\<Gamma>, if b then e1 else e2, S)" 
+    have "consistent (ae, ce, a', as', r) (\<Gamma>, if b then e1 else e2, S)" 
       using if\<^sub>2 by (auto dest!: a_consistent_if\<^sub>2)
     }
     moreover
-    have "conf_transform (ae, ce, a, as) (\<Gamma>, Bool b, Alts e1 e2 # S) \<Rightarrow>\<^sub>G conf_transform (ae, ce, a', as') (\<Gamma>, if b then e1 else e2, S)"
+    have "conf_transform (ae, ce, a, as, r) (\<Gamma>, Bool b, Alts e1 e2 # S) \<Rightarrow>\<^sub>G conf_transform (ae, ce, a', as', r) (\<Gamma>, if b then e1 else e2, S)"
       by (auto intro:normal  step.if\<^sub>2[where b = True, simplified] step.if\<^sub>2[where b = False, simplified])
     ultimately
     show ?case by (blast del: consistentI consistentE)
   next
-    case refl thus ?case by auto
+    case refl thus ?case by force
   next
     case (trans c c' c'')
       from trans(3)[OF trans(5)]
-      obtain ae' ce' a' as' where "consistent (ae', ce', a', as') c'" and *: "conf_transform (ae, ce, a, as) c \<Rightarrow>\<^sub>G\<^sup>* conf_transform (ae', ce', a', as') c'" by blast
+      obtain ae' ce' a' as' r'
+      where "consistent (ae', ce', a', as', r') c'" and *: "conf_transform (ae, ce, a, as, r) c \<Rightarrow>\<^sub>G\<^sup>* conf_transform (ae', ce', a', as', r') c'" by blast
       from trans(4)[OF this(1)]
-      obtain ae'' ce'' a'' as'' where "consistent (ae'', ce'', a'', as'') c''" and **: "conf_transform (ae', ce', a', as') c' \<Rightarrow>\<^sub>G\<^sup>* conf_transform (ae'', ce'', a'', as'') c''" by blast
+      obtain ae'' ce'' a'' as'' r''
+      where "consistent (ae'', ce'', a'', as'', r'') c''" and **: "conf_transform (ae', ce', a', as', r') c' \<Rightarrow>\<^sub>G\<^sup>* conf_transform (ae'', ce'', a'', as'', r'') c''" by blast
       from this(1) rtranclp_trans[OF * **]
       show ?case by blast
   qed
