Launchbury/SestoftGC.thy
@@ -2,14 +2,13 @@ theory SestoftGC
 imports Sestoft 
 begin
 
-inductive gc_step :: "conf \<Rightarrow> conf \<Rightarrow> bool" (infix "\<Rightarrow>\<^sub>G" 50) where
-  normal:  "c \<Rightarrow> c' \<Longrightarrow> c \<Rightarrow>\<^sub>G c'"
-| drop:    "(\<Gamma>, e, S) \<Rightarrow>\<^sub>G (restrictA V \<Gamma>, e, S)"
-| dropUpd: "(\<Gamma>, e, Upd x # S) \<Rightarrow>\<^sub>G (\<Gamma>, e, S)"
+inductive gc_step :: "(var list \<times> conf) \<Rightarrow> (var list \<times> conf) \<Rightarrow> bool" (infix "\<Rightarrow>\<^sub>G" 50) where
+  normal:  "c \<Rightarrow> c' \<Longrightarrow> (r, c) \<Rightarrow>\<^sub>G (r, c')"
+| dropUpd: "(r, \<Gamma>, e, Upd x # S) \<Rightarrow>\<^sub>G (x # r, \<Gamma>, e, S)"
 
 lemmas gc_step_intros[intro] =
   normal[OF step.intros(1)] normal[OF step.intros(2)] normal[OF step.intros(3)]
-  normal[OF step.intros(4)] normal[OF step.intros(5)] drop dropUpd
+  normal[OF step.intros(4)] normal[OF step.intros(5)]  dropUpd
 
 
 abbreviation gc_steps (infix "\<Rightarrow>\<^sub>G\<^sup>*" 50) where "gc_steps \<equiv> gc_step\<^sup>*\<^sup>*"
@@ -17,36 +16,299 @@ lemmas converse_rtranclp_into_rtranclp[of gc_step, OF _ r_into_rtranclp, trans]
 
 lemma var_onceI:
   assumes "map_of \<Gamma> x = Some e"
-  shows "(\<Gamma>, Var x, S) \<Rightarrow>\<^sub>G\<^sup>* (delete x \<Gamma>, e , S)"
+  shows "(r, \<Gamma>, Var x, S) \<Rightarrow>\<^sub>G\<^sup>* (x#r, delete x \<Gamma>, e , S)"
 proof-
   from assms 
-  have "(\<Gamma>, Var x, S) \<Rightarrow>\<^sub>G (delete x \<Gamma>, e , Upd x # S)"..
+  have "(r, \<Gamma>, Var x, S) \<Rightarrow>\<^sub>G (r, delete x \<Gamma>, e , Upd x # S)"..
   moreover
-  have "\<dots> \<Rightarrow>\<^sub>G  (delete x \<Gamma>, e , S)"..
+  have "\<dots> \<Rightarrow>\<^sub>G  (x #r, delete x \<Gamma>, e , S)"..
   ultimately
   show ?thesis by (rule converse_rtranclp_into_rtranclp[OF _ r_into_rtranclp])
 qed
 
-lemma let_and_restrict:
-  assumes "atom ` domA \<Delta> \<sharp>* \<Gamma>" and "atom ` domA \<Delta> \<sharp>* S"
-  assumes "V \<subseteq> domA \<Delta>"
-  shows "(\<Gamma>, Let \<Delta> e, S) \<Rightarrow>\<^sub>G\<^sup>* (restrictA V \<Delta> @ \<Gamma>, e, S)"
+lemma normal_trans:  "c \<Rightarrow>\<^sup>* c' \<Longrightarrow> (r, c) \<Rightarrow>\<^sub>G\<^sup>* (r, c')"
+  by (induction rule:rtranclp_induct)
+     (simp, metis normal rtranclp.rtrancl_into_rtrancl)
+
+fun to_gc_conf :: "var list \<Rightarrow> conf \<Rightarrow> conf"
+  where "to_gc_conf r (\<Gamma>, e, S) = (restrictA (- set r) \<Gamma>, e, restr_stack (- set r) S)"
+
+lemma to_gc_conf_append[simp]:
+  "to_gc_conf (r@r') c = to_gc_conf r (to_gc_conf r' c)"
+  by (cases c) auto
+
+lemma to_gc_conf_eqE[elim!]:
+  assumes  "to_gc_conf r c = (\<Gamma>, e, S)"
+  obtains \<Gamma>' S' where "c = (\<Gamma>', e, S')" and "\<Gamma> = restrictA (- set r) \<Gamma>'" and "S = restr_stack (- set r) S'"
+  using assms
+  by (cases c) auto
+
+fun safe_hd :: "'a list \<Rightarrow> 'a option"
+ where  "safe_hd (x#_) = Some x"
+     |  "safe_hd [] = None"
+
+lemma safe_hd_None[simp]: "safe_hd xs = None \<longleftrightarrow> xs = []"
+  by (cases xs) auto
+
+abbreviation r_ok :: "(var list \<times> conf) \<Rightarrow> bool"
+  where "r_ok c \<equiv> set (fst c) \<subseteq> domA (fst (snd c)) \<union> upds (snd (snd (snd c)))"
+
+
+lemma sestoftUnGCStack:
+  assumes "heap_upds_ok (\<Gamma>, S)"
+  assumes "set r \<subseteq> domA \<Gamma> \<union> upds S"
+  obtains \<Gamma>' S' where
+    "(\<Gamma>, e, S) \<Rightarrow>\<^sup>* (\<Gamma>', e, S')"
+    "heap_upds_ok (\<Gamma>', S')"
+    "to_gc_conf r (\<Gamma>, e, S) = to_gc_conf r (\<Gamma>', e, S')"
+    "\<not> isVal e \<or> safe_hd S' = safe_hd (restr_stack (- set r) S')"
+    "set r \<subseteq> domA \<Gamma>' \<union> upds S'"
+(*proof(atomize_elim)
+  show "\<exists>\<Gamma>' S'. (\<Gamma>, e, S) \<Rightarrow>\<^sup>* (\<Gamma>', e, S') \<and> heap_upds_ok (\<Gamma>', S') \<and> to_gc_conf r (\<Gamma>, e, S) = to_gc_conf r (\<Gamma>', e, S') \<and> (\<not> isVal e \<or>  safe_hd S' = safe_hd (restr_stack (- set r) S'))"
+*)
 proof-
-  from assms(1,2) have "(\<Gamma>, Let \<Delta> e, S) \<Rightarrow>\<^sub>G (\<Delta> @ \<Gamma>, e, S)"..
-  also
-  have "\<dots> \<Rightarrow>\<^sub>G (restrictA (V \<union> domA \<Gamma>) (\<Delta> @ \<Gamma>), e, S)"..
-  also
-  from fresh_distinct[OF assms(1)]
-  have "restrictA (V \<union> domA \<Gamma>) \<Delta> = restrictA V \<Delta>" by (induction \<Delta>) auto
-  hence "restrictA (V \<union> domA \<Gamma>) (\<Delta> @ \<Gamma>) = restrictA V \<Delta> @ \<Gamma>"
-    by (simp add: restrictA_append restrictA_noop)
-  finally show ?thesis.
+  show ?thesis
+  proof(cases "isVal e")
+    case False
+    thus ?thesis using assms  by -(rule that, auto)
+  next
+    case True
+    from that assms 
+    show ?thesis
+    apply (atomize_elim)
+    proof(induction S arbitrary: \<Gamma>)
+      case Nil thus ?case by (fastforce)
+    next
+      case (Cons s S)
+      show ?case
+      proof(cases "Some s = safe_hd (restr_stack (- set r) (s#S))")
+        case True
+        thus ?thesis
+          using `isVal e` `heap_upds_ok (\<Gamma>, s # S)` `set r \<subseteq> domA \<Gamma> \<union> upds (s # S)`
+          apply auto
+          apply (intro exI conjI)
+          apply (rule rtranclp.intros(1))
+          apply auto
+          done
+      next
+        case False
+        then obtain x where [simp]: "s = Upd x" and [simp]: "x \<in> set r"
+          by(cases s) (auto split: if_splits)
+      
+        from `heap_upds_ok (\<Gamma>, s # S)` `s = Upd x`
+        have [simp]: "x \<notin> domA \<Gamma>" and "heap_upds_ok ((x,e) # \<Gamma>, S)"
+          by (auto dest: heap_upds_okE) 
+
+        from `set r \<subseteq> domA \<Gamma> \<union> upds (s # S)`
+        have "set r \<subseteq> domA ((x,e) # \<Gamma>) \<union> upds S" by auto
+        
+        have "(\<Gamma>, e, s # S) \<Rightarrow>\<^sup>* (\<Gamma>, e, Upd x # S)" unfolding `s = _` ..
+        also have "\<dots> \<Rightarrow> ((x,e) # \<Gamma>, e, S)" by (rule var\<^sub>2[OF `x \<notin> domA \<Gamma>` `isVal e`])
+        also
+        from Cons.IH[OF `heap_upds_ok ((x,e) # \<Gamma>, S)`  `set r \<subseteq> domA ((x,e) # \<Gamma>) \<union> upds S`]
+        obtain \<Gamma>' S' where  "((x,e) # \<Gamma>, e, S) \<Rightarrow>\<^sup>* (\<Gamma>', e, S')"
+            and res: "heap_upds_ok (\<Gamma>', S')"
+                     "to_gc_conf r ((x,e) # \<Gamma>, e, S) = to_gc_conf r (\<Gamma>', e, S')"
+                     "(\<not> isVal e \<or> safe_hd S' = safe_hd (restr_stack (- set r) S'))"
+                     "set r \<subseteq> domA \<Gamma>' \<union> upds S'"
+          by blast
+        note this(1)
+        finally
+        have "(\<Gamma>, e, s # S) \<Rightarrow>\<^sup>* (\<Gamma>', e, S')".
+        thus ?thesis  using res by auto
+      qed
+    qed
+  qed
 qed
-    
   
 
-lemma normal_trans:  "c \<Rightarrow>\<^sup>* c' \<Longrightarrow> c \<Rightarrow>\<^sub>G\<^sup>* c'"
-  by (induction rule:rtranclp_induct) (auto dest: normal)
+lemma sestoftUnGCstep:
+  assumes "to_gc_conf r c \<Rightarrow> d"
+  assumes "heap_upds_ok_conf c"
+  assumes "r_ok (r, c)"
+  shows   "\<exists> c'. c \<Rightarrow>\<^sup>* c' \<and> d = to_gc_conf r c' \<and> heap_upds_ok_conf c' \<and> r_ok (r, c')"
+proof-
+  obtain \<Gamma> e S where "c = (\<Gamma>, e, S)" by (cases c) auto
+  with assms
+  have "heap_upds_ok (\<Gamma>,S)" and "set r \<subseteq> domA \<Gamma> \<union> upds S" by auto
+  from sestoftUnGCStack[OF this]
+  obtain \<Gamma>' S' where
+    "(\<Gamma>, e, S) \<Rightarrow>\<^sup>* (\<Gamma>', e, S')"
+    and *: "to_gc_conf r (\<Gamma>, e, S) = to_gc_conf r (\<Gamma>', e, S')"
+    and disj: "\<not> isVal e \<or> safe_hd S' = safe_hd (restr_stack (- set r) S')"
+    and "heap_upds_ok (\<Gamma>', S')"
+    and "set r \<subseteq> domA \<Gamma>' \<union> upds S'" by metis
+  note this(1)
+  also
+
+  from assms(1)[unfolded `c =_ ` *]
+  have "\<exists> \<Gamma>'' e'' S''. (\<Gamma>', e, S') \<Rightarrow> (\<Gamma>'', e'', S'')  \<and> d = to_gc_conf r (\<Gamma>'', e'', S'') \<and> heap_upds_ok (\<Gamma>'', S'') \<and> set r \<subseteq> domA \<Gamma>'' \<union> upds S''"
+  proof(cases rule: step.cases)
+    case app\<^sub>1
+    thus ?thesis
+      using `heap_upds_ok (\<Gamma>', S')` and `set r \<subseteq> domA \<Gamma>' \<union> upds S'`
+      apply auto
+      apply (intro exI conjI)
+      apply (rule step.intros)
+      apply auto
+      done
+  next
+    case app\<^sub>2
+    thus ?thesis
+      using disj  `heap_upds_ok (\<Gamma>', S')` `set r \<subseteq> domA \<Gamma>' \<union> upds S'`
+      apply (cases S')
+      apply auto
+      apply (intro exI conjI)
+      apply (rule step.intros)
+      apply auto
+      done
+  next
+    case var\<^sub>1
+    thus ?thesis
+      using `heap_upds_ok (\<Gamma>', S')` `set r \<subseteq> domA \<Gamma>' \<union> upds S'`
+      apply auto
+      apply (intro exI conjI)
+      apply (rule step.intros)
+      apply (auto simp add: restr_delete_twist)
+      done
+  next
+    case var\<^sub>2
+    thus ?thesis
+      using disj `heap_upds_ok (\<Gamma>', S')` `set r \<subseteq> domA \<Gamma>' \<union> upds S'`
+      apply (cases S')
+      apply auto
+      apply (intro exI conjI)
+      apply (rule step.intros)
+      apply (auto split: if_splits dest: Upd_eq_restr_stackD2)
+      done
+  next
+    case (let\<^sub>1 \<Delta>'' \<Gamma>'' S'' e')
+    thus ?thesis
+      using `heap_upds_ok (\<Gamma>', S')` `set r \<subseteq> domA \<Gamma>' \<union> upds S'`
+      apply auto
+      apply (intro exI conjI)
+      apply (rule step.intros)
+      apply (auto simp add: restrictA_append)
+      sorry
+  next
+    case if\<^sub>1
+    thus ?thesis
+      using `heap_upds_ok (\<Gamma>', S')` `set r \<subseteq> domA \<Gamma>' \<union> upds S'`
+      apply auto
+      apply (intro exI conjI)
+      apply (rule step.intros)
+      apply (auto)
+      done
+  next
+    case if\<^sub>2
+    thus ?thesis
+      using disj `heap_upds_ok (\<Gamma>', S')` `set r \<subseteq> domA \<Gamma>' \<union> upds S'`
+      apply (cases S')
+      apply auto
+      apply (intro exI conjI)
+      apply (rule step.if\<^sub>2[where b = True, simplified] step.if\<^sub>2[where b = False, simplified])
+      apply (auto split: if_splits dest: Upd_eq_restr_stackD2)
+      apply (intro exI conjI)
+      apply (rule step.if\<^sub>2[where b = True, simplified] step.if\<^sub>2[where b = False, simplified])
+      apply (auto split: if_splits dest: Upd_eq_restr_stackD2)
+      done
+  qed
+  then obtain \<Gamma>'' e'' S''
+    where "(\<Gamma>', e, S') \<Rightarrow> (\<Gamma>'', e'', S'')"
+    and "d = to_gc_conf r (\<Gamma>'', e'', S'')"
+    and "heap_upds_ok (\<Gamma>'', S'')"
+    and "set r \<subseteq> domA \<Gamma>'' \<union> upds S''"
+    by blast
+  note this(1)
+  finally
+  have "(\<Gamma>, e, S) \<Rightarrow>\<^sup>* (\<Gamma>'', e'', S'')".
+  with `d = _` `heap_upds_ok (\<Gamma>'', S'')` `set r \<subseteq> domA \<Gamma>'' \<union> upds S''`
+  show ?thesis unfolding `c = _` by auto
+qed
+
+
+lemma sestoftUnGC:
+  assumes "(r, to_gc_conf r c) \<Rightarrow>\<^sub>G\<^sup>* (r', d)" and "heap_upds_ok_conf c" and "r_ok (r, c)"
+  shows   "\<exists> c'. c \<Rightarrow>\<^sup>* c' \<and> d = to_gc_conf r' c' \<and> heap_upds_ok_conf c' \<and> r_ok (r', c')"
+using assms
+proof(induction r' "d"  rule: rtranclp_induct2)
+  case refl
+  thus ?case by blast
+next
+  case (step r' d' r'' d'')
+  then obtain c' where "c \<Rightarrow>\<^sup>* c'" and "d' = to_gc_conf r' c'" and "heap_upds_ok_conf c'" and "r_ok (r', c')" by auto
+  with step
+  have "(r', to_gc_conf r' c') \<Rightarrow>\<^sub>G (r'', d'')" by simp
+  hence "\<exists> c''. c' \<Rightarrow>\<^sup>* c'' \<and> d'' = to_gc_conf r'' c'' \<and> heap_upds_ok_conf c'' \<and> r_ok (r'', c'')"
+  proof(cases rule: gc_step.cases)
+    case normal
+    from sestoftUnGCstep[OF normal(2) `heap_upds_ok_conf c'` `r_ok (r',c')`] `r'' = r'`
+    show ?thesis by auto
+  next
+    case (dropUpd \<Gamma> e x S)
+    from `to_gc_conf r' c' = (\<Gamma>, e, Upd x # S)`
+    have "x \<notin> set r'" by (auto dest: Upd_eq_restr_stackD)
+    
+    from `heap_upds_ok_conf c'` and `to_gc_conf r' c' = (\<Gamma>, e, Upd x # S)`
+    have "heap_upds_ok (\<Gamma>, Upd x # S)" by fastforce
+    hence [simp]: "x \<notin> domA \<Gamma>" "x \<notin> upds S" by (auto dest: heap_upds_ok_upd)
+
+    from `to_gc_conf r' c' = (\<Gamma>, e, Upd x # S)`
+    have "Upd x # S = restr_stack (- set r') (snd (snd c'))"  by auto
+    from arg_cong[where f = upds, OF this]
+    have "x \<in> upds (snd (snd c'))" by auto
+    with `r_ok (r', c')` have "r_ok (x # r', c')" by auto
+
+    have "to_gc_conf (x # r') c' = to_gc_conf ([x]@ r') c'" by simp
+    also have "\<dots> = to_gc_conf [x] (to_gc_conf r' c')" by (rule to_gc_conf_append)
+    also have "\<dots> = to_gc_conf [x] (\<Gamma>, e, Upd x # S)" unfolding `to_gc_conf r' c' = _`..
+    also have "\<dots> = (\<Gamma>, e, S)" by (auto intro: restrictA_noop)
+    finally have "to_gc_conf (x # r') c' = (\<Gamma>, e, S)".
+    with dropUpd  `heap_upds_ok_conf c'` `r_ok (x # r', c')`
+    show ?thesis by fastforce
+  qed
+  then obtain c'' where "c' \<Rightarrow>\<^sup>* c''" and "d'' = to_gc_conf r'' c''" and "heap_upds_ok_conf c''" and "r_ok (r'', c'')" by auto
+  with `c \<Rightarrow>\<^sup>* c'` `c' \<Rightarrow>\<^sup>* c''`
+  have "c \<Rightarrow>\<^sup>* c''" by auto
+  with `d'' = _` `heap_upds_ok_conf c''` `r_ok (r'', c'')`
+  show ?case by blast
+qed
+  
+lemma sestoftUnGC':
+  assumes "([], [], e, []) \<Rightarrow>\<^sub>G\<^sup>* (r, \<Gamma>, e', [])"
+  assumes "isVal e'"
+  shows   "\<exists> \<Gamma>''. ([], e, []) \<Rightarrow>\<^sup>* (\<Gamma>'', e', []) \<and> \<Gamma> = restrictA (- set r) \<Gamma>'' \<and> set r \<subseteq> domA \<Gamma>''"
+proof-
+ from sestoftUnGC[where r = "[]" and c = "([], e, [])", simplified, OF assms(1)]
+ obtain \<Gamma>' S'
+  where "([], e, []) \<Rightarrow>\<^sup>* (\<Gamma>', e', S')"
+    and "\<Gamma> = restrictA (- set r) \<Gamma>'"
+    and "restr_stack (- set r) S' = []"
+    and "heap_upds_ok (\<Gamma>', S')"
+    and "set r \<subseteq> domA \<Gamma>' \<union> upds S'"
+    by auto
+ 
+  from `isVal e'` sestoftUnGCStack[where e = e', OF `heap_upds_ok (\<Gamma>', S')` `set r \<subseteq> domA \<Gamma>' \<union> upds S'`]
+  obtain \<Gamma>'' S''
+    where "(\<Gamma>', e', S') \<Rightarrow>\<^sup>* (\<Gamma>'', e', S'')"
+    and   "heap_upds_ok (\<Gamma>'', S'')"
+    and "to_gc_conf r (\<Gamma>', e', S') = to_gc_conf r (\<Gamma>'', e', S'')"
+    and "safe_hd S'' = safe_hd (restr_stack (- set r) S'')"
+    and "set r \<subseteq> domA \<Gamma>'' \<union> upds S''"
+    by metis
+  from this (3,4) `restr_stack (- set r) S' = []`
+  have "S'' = []" by auto
+ 
+  from `([], e, []) \<Rightarrow>\<^sup>* (\<Gamma>', e', S')` and `(\<Gamma>', e', S') \<Rightarrow>\<^sup>* (\<Gamma>'', e', S'')` and `S'' = []`
+  have "([], e, []) \<Rightarrow>\<^sup>* (\<Gamma>'', e', [])" by auto
+  moreover
+  have "\<Gamma> = restrictA (- set r) \<Gamma>''" using `to_gc_conf r _ = _` `\<Gamma> = _` by auto
+  moreover
+  from `set r \<subseteq> domA \<Gamma>'' \<union> upds S''` `S'' = []`
+  have "set r \<subseteq> domA \<Gamma>''" by simp
+  ultimately
+  show ?thesis by blast
+qed
 
 
 end
